Finish the inlining

proofmode/HPSim.v
@@ -22,8 +22,6 @@ Require Import ProofMode Invariant.
 
 Require Import HTactics.
 
-
-
 Section SIM.
 
 	Context `{Σ: GRA.t}.
@@ -65,10 +63,10 @@ Section SIM.
 	| hpsim_call
 			f_src f_tgt st_src st_tgt fmr
 			fn varg k_src k_tgt FR
-      (INV: Own fmr ⊢ #=> (I st_src st_tgt ** FR))
+                        (INV: Own fmr ⊢ #=> (I st_src st_tgt ** FR))
 			(K: forall vret st_src0 st_tgt0 fmr0 
 					(WF: URA.wf fmr0)
-          (INV: Own fmr0 ⊢ #=> (I st_src0 st_tgt0 ** FR)),
+                                        (INV: Own fmr0 ⊢ #=> (I st_src0 st_tgt0 ** FR)),
 				_hpsim hpsim true true (st_src0, k_src vret) (st_tgt0, k_tgt vret) fmr0)				
 		:
 			_hpsim hpsim f_src f_tgt (st_src, trigger (Call fn varg) >>= k_src) (st_tgt, trigger (Call fn varg) >>= k_tgt) fmr
@@ -85,7 +83,7 @@ Section SIM.
 			f_src f_tgt st_src st_tgt fmr
 			fn f varg k_src i_tgt
 			(FUN: alist_find fn fl_src = Some f)
-			(K: _hpsim hpsim true f_tgt (st_src, (f varg) >>= k_src) (st_tgt, i_tgt) fmr)
+			(K: _hpsim hpsim true f_tgt (st_src, x <- f varg ;; trigger (Guarantee (True%I)) ;;; k_src x) (st_tgt, i_tgt) fmr)
 		:
 			_hpsim hpsim f_src f_tgt (st_src, trigger (Call fn varg) >>= k_src) (st_tgt, i_tgt) fmr
 
@@ -93,7 +91,7 @@ Section SIM.
 			f_src f_tgt st_src st_tgt fmr
 			fn f varg i_src k_tgt
 		  (FUN: alist_find fn fl_tgt = Some f)
-		  (K: _hpsim hpsim f_src true (st_src, i_src) (st_tgt, (f varg) >>= k_tgt) fmr)
+		  (K: _hpsim hpsim f_src true (st_src, i_src) (st_tgt, x <- f varg ;; trigger (Guarantee (True%I)) ;;; k_tgt x) fmr)
 	  :
 		  _hpsim hpsim f_src f_tgt (st_src, i_src) (st_tgt, trigger (Call fn varg) >>= k_tgt) fmr
 
@@ -214,6 +212,7 @@ Section SIM.
 		Hint Resolve _hpsim_mon: paco.
 		Hint Resolve cpn5_wcompat: paco.
 
+(*                
 		Lemma hpsim_ind
 				(P: bool -> bool -> Any.t * itree hAGEs Any.t -> Any.t * itree hAGEs Any.t -> Σ -> Prop)
 		
@@ -370,7 +369,8 @@ Section SIM.
 			{ eapply GUARANTEETGT; eauto. i. hexploit K; et. i. des. esplits; et. }
 			{ eapply PROGRESS; eauto. pclearbot. et. }
 	Qed.
-
+ *)
+                
 	Lemma hpsim_bot_flag_up f_src f_tgt st_src st_tgt fmr
 			(SIM: paco5 _hpsim bot5 true true st_src st_tgt fmr)
 		:
@@ -534,29 +534,6 @@ Section SIM.
     eapply current_iProp_entail; eauto.
   Qed.
 
-  (* Move to HoareDef. *)
-  Lemma interp_hp_Assume iP fr
-  :
-  (interp_hp (trigger (Assume iP)) fr)
-  =
-  (* interp_state (handle_hAGE_tgt) (trigger (Assume iP)) fr *)
-  ('(fr, _) <- (handle_Assume iP fr);; tau;; Ret (fr, tt))
-  .
-  Proof.
-    unfold interp_hp, trigger. rewrite ! interp_state_vis. grind. rewrite u. et.
-  Qed.
-
-  Lemma interp_hp_Guarantee iP fr
-  :
-  (interp_hp (trigger (Guarantee iP)) fr)
-  =
-  (* interp_state (handle_hAGE_tgt) (trigger (Assume iP)) fr *)
-  ('(fr', _) <- (handle_Guarantee iP fr);; tau;; Ret (fr', tt))
-  .
-  Proof.
-    unfold interp_hp, trigger. rewrite ! interp_state_vis. grind. rewrite u. et.
-  Qed.
-
   (* Variable st: Any.t.
      Variable frr: Σ.
      Variable itr: Σ -> itree Es (Σ * Any.t).
@@ -569,197 +546,826 @@ Section SIM.
 
   (* Variable world: Type. *)
 
-
-  Section INLINEC.
-    (* Check (@_sim_itree Σ wf le fl_src' fl_tgt'). *)
-
-    Inductive interp_hp_le: (Σ*Any.t -> itree Es Any.t) -> (Σ*Any.t -> itree Es Any.t) -> Prop :=
-    | interp_hp_le_base
-      :
-      interp_hp_le hp_fun_tail hp_fun_tail
-    | interp_hp_le_same
-        ktrH ktr1 ktr2
-        (KEQV: interp_hp_le ktr1 ktr2)
-      :
-      interp_hp_le (fun '(fr,x) => interp_hp (ktrH x) fr >>= ktr1) (fun '(fr,x) => interp_hp (ktrH x) fr >>= ktr2)
-    | interp_hp_le_inc
-        ktr1 ktr2
-        (KEQV: interp_hp_le ktr1 ktr2)
-      :
-      interp_hp_le ktr1 (fun frx => hp_fun_tail frx >>= (fun x => tau;; Ret (ε,x)) >>= ktr2)
-    .
-
-    Variant inlineC
-      (r: forall S_src S_tgt (SS: Any.t -> Any.t -> S_src -> S_tgt -> Prop), bool -> bool -> Σ -> Any.t * itree Es S_src -> Any.t * itree Es S_tgt -> Prop):
-      forall S_src S_tgt (SS: Any.t -> Any.t -> S_src -> S_tgt -> Prop), bool -> bool -> Σ -> Any.t * itree Es S_src -> Any.t * itree Es S_tgt -> Prop :=
-    | inlineSrcC_intro SS f_src f_tgt w
-	st_src st_tgt (fr_src mr_src fr_src' mr_src' fr_tgt mr_tgt fr_tgt' mr_tgt': Σ)
-        ktr_src ktr_src' ktr_tgt ktr_tgt' x
-        (EQ_src: fr_src ⋅ mr_src = fr_src' ⋅ mr_src')
-        (EQ_tgt: fr_src ⋅ mr_src = fr_src' ⋅ mr_src')
-        (LE_src: interp_hp_le ktr_src ktr_src')
-        (LE_tgt: interp_hp_le ktr_tgt ktr_tgt')
-	(SIM: r Any.t Any.t SS f_src f_tgt w (Any.pair st_src mr_src↑, ktr_src (fr_src,x)) (Any.pair st_tgt mr_tgt↑, ktr_tgt (fr_tgt,x)))
-      :
-      inlineC r Any.t Any.t SS f_src f_tgt w (Any.pair st_src mr_src'↑, ktr_src' (fr_src',x)) (Any.pair st_tgt mr_tgt'↑, ktr_tgt' (fr_tgt',x))
-    .
-    Hint Constructors inlineC: core.
-
-    Lemma inlineC_mon r1 r2
-      (LEr: r1 <8= r2)
+  Variant _sim_strict (sim_strict: forall R, relation (Any.t * R) -> relation (Any.t * itree Es R))
+    : forall R, relation (Any.t * R) -> relation (Any.t * itree Es R)
+  :=
+  | sim_strict_ret R RR st st' v v'
+      (RET: RR (st,v) (st',v'): Prop)
     :
-    inlineC r1 <8= inlineC r2
+    _sim_strict sim_strict R RR
+      (st, Ret v)
+      (st', Ret v')
+  | sim_strict_call R RR
+      st fn varg k k'
+      (K: forall st0 vret,
+          sim_strict R RR (st0, k vret) (st0, k' vret))
+    :
+    _sim_strict sim_strict R RR
+      (st, trigger (Call fn varg) >>= k)
+      (st, trigger (Call fn varg) >>= k')
+  | sim_strict_syscall R RR
+      st st' fn varg rvs k k'
+      (K: forall vret,
+          sim_strict R RR (st, k vret) (st', k' vret))
+    :
+    _sim_strict sim_strict R RR
+      (st, trigger (Syscall fn varg rvs) >>= k)
+      (st', trigger (Syscall fn varg rvs) >>= k')
+  | sim_strict_tau R RR
+      st st' i i'
+      (K: sim_strict R RR (st, i) (st', i'))
+    :
+    _sim_strict sim_strict R RR
+      (st, tau;; i)
+      (st', tau;; i')
+  | sim_strict_choose R RR
+      st st' X X' k k'
+      (K: forall x', exists x, sim_strict R RR (st, k x) (st', k' x'))
+    :
+    _sim_strict sim_strict R RR
+      (st, trigger (Choose X) >>= k)
+      (st', trigger (Choose X') >>= k')
+  | sim_strict_take R RR
+      st st' X X' k k'
+      (K: forall x, exists x', sim_strict R RR (st, k x) (st', k' x'))
+    :
+    _sim_strict sim_strict R RR
+      (st, trigger (Take X) >>= k)
+      (st', trigger (Take X') >>= k')
+  | sim_strict_supdate R RR
+      st st' X k X' k' (run: Any.t -> Any.t * X) (run': Any.t -> Any.t * X')
+      (K: sim_strict R RR
+            (fst (run st), k (snd (run st)))
+            (fst (run' st'), k' (snd (run' st'))))
+    :
+    _sim_strict sim_strict R RR
+      (st, trigger (SUpdate run) >>= k)
+      (st', trigger (SUpdate run') >>= k')
+  .
+
+  Definition sim_strict := paco4 _sim_strict bot4.
+
+  Lemma sim_strict_mon: monotone4 _sim_strict.
+  Proof.
+    ii. induction IN; try (econs; et; ii; exploit K; i; des; et).
+  Qed.
+
+  Hint Constructors _sim_strict.
+  Hint Unfold sim_strict.
+  Hint Resolve sim_strict_mon: paco.
+  Hint Resolve cpn4_wcompat: paco.
+
+  Lemma sim_strict_refl
+    R sti
+    :
+    sim_strict R eq sti sti.
+  Proof.
+    revert_until I. ginit. gcofix CIH; i.
+    destruct sti as [st i]. ides i; eauto with paco.
+    gstep. destruct e; [destruct c|destruct s; [destruct s|destruct e]].
+    - hexploit (sim_strict_call (gpaco4 _sim_strict (cpn4 _sim_strict) r r) R eq); i.
+      { instantiate (1:=k). eauto with paco. }
+      unfold trigger in H. rewrite !bind_vis in H.
+      erewrite f_equal2; eauto; repeat (eapply f_equal; eauto);
+        extensionality x; rewrite !bind_ret_l; eauto.
+    - hexploit (sim_strict_supdate (gpaco4 _sim_strict (cpn4 _sim_strict) r r) R eq); i.
+      { instantiate (4:=k). eauto with paco. }
+      unfold trigger in H. rewrite !bind_vis in H.
+      erewrite f_equal2; eauto; repeat (eapply f_equal; eauto);
+        extensionality x; rewrite !bind_ret_l; eauto.
+    - hexploit (sim_strict_choose (gpaco4 _sim_strict (cpn4 _sim_strict) r r) R eq); i.
+      { eexists. instantiate (4:=k). eauto with paco. }
+      unfold trigger in H. rewrite !bind_vis in H.
+      erewrite f_equal2; eauto; repeat (eapply f_equal; eauto);
+        extensionality x; rewrite !bind_ret_l; eauto.
+    - hexploit (sim_strict_take (gpaco4 _sim_strict (cpn4 _sim_strict) r r) R eq); i.
+      { eexists. instantiate (4:=k). eauto with paco. }
+      unfold trigger in H. rewrite !bind_vis in H.
+      erewrite f_equal2; eauto; repeat (eapply f_equal; eauto);
+        extensionality x; rewrite !bind_ret_l; eauto.
+    - hexploit (sim_strict_syscall (gpaco4 _sim_strict (cpn4 _sim_strict) r r) R eq); i.
+      { instantiate (3:=k). eauto with paco. }
+      unfold trigger in H. rewrite !bind_vis in H.
+      erewrite f_equal2; eauto; repeat (eapply f_equal; eauto);
+        extensionality x; rewrite !bind_ret_l; eauto.
+  Qed.
+
+  Lemma sim_strict_le
+    R RR RR'
+    (LE: RR <2= RR')
+    :
+    sim_strict R RR <2= sim_strict R RR'.
+  Proof.
+    ginit. gcofix CIH. i. punfold PR.
+    inv PR; grind; depdes H0; unfold trigger in *;
+      try (rewrite !bind_vis in x); gstep; econs; i;
+      try edestruct K; pclearbot; eauto with paco.
+  Qed.
+
+  Variant sim_strict_bindC (r: forall R, relation (Any.t*R) -> relation (Any.t * itree Es R)) :
+    forall R, relation (Any.t*R) -> relation (Any.t * itree Es R)
+  :=
+  | sim_strict_bindC_intro R RR Q QQ st st' i i' k k'
+      (HD: r R RR (st,i) (st',i'))
+      (TL: forall st0 v0 st0' v0' (REL: RR (st0,v0) (st0',v0')),
+           r Q QQ (st0, k v0) (st0', k' v0'))
+    :
+    sim_strict_bindC r Q QQ (st, i >>= k) (st', i' >>= k')
+  .
+
+  Lemma sim_strict_bindC_mon
+        r1 r2
+        (LEr: r1 <4= r2)
+    :
+    sim_strict_bindC r1 <4= sim_strict_bindC r2
   .
   Proof. ii. destruct PR; econs; et. Qed.
 
-  Lemma inlineC_compatible: forall wf le fl_src fl_tgt, 
-      compatible8 (@_sim_itree Σ wf le fl_src fl_tgt) inlineC.
+  Lemma sim_strict_bindC_wrespectful:
+    wrespectful4 _sim_strict sim_strict_bindC.
   Proof.
-    econs; i; eauto using inlineC_mon.
-    depdes PR.
-    remember (Any.pair st_src mr_src↑, ktr_src (fr_src,x)) as sitr_src.
-    remember (Any.pair st_tgt mr_tgt↑, ktr_tgt (fr_tgt,x)) as sitr_tgt.
-    move SIM before r. revert_until SIM.
-    induction SIM; i; depdes Heqsitr_src; depdes Heqsitr_tgt.
-    - exfalso. clear EQ_src EQ_tgt x. revert fr_src x0 x1. induction LE_src; i; eauto.
-      + admit.
-      + admit.
+    econs; eauto using sim_strict_bindC_mon; i.
+    destruct PR. apply GF in HD. inv HD; grind; depdes H3 H0; grind;
+      try (by econs; i; econs 2; eauto; econs; eauto using rclo4).
+    - eapply sim_strict_mon; eauto using rclo4.
+    - econs. i. specialize (K x'). des.
+      eexists. econs 2; eauto. econs; eauto using rclo4.
+    - econs. i. specialize (K x). des.
+      eexists. econs 2; eauto. econs; eauto using rclo4.
+  Qed.
+
+  Lemma sim_strict_bindC_spec:
+    sim_strict_bindC <5= gupaco4 _sim_strict (cpn4 _sim_strict).
+  Proof.
+    intros. eapply wrespect4_uclo; eauto with paco.
+    apply sim_strict_bindC_wrespectful.
+  Qed.
+
+  Variant sim_strict_transC (r: forall R, relation (Any.t*R) -> relation (Any.t * itree Es R)) :
+    forall R, relation (Any.t*R) -> relation (Any.t * itree Es R)
+  :=
+  | sim_strict_transC_intro R RR0 RR1 RR st st' st'' i i' i''
+      (REL0: r R RR0 (st,i) (st',i'))
+      (REL1: r R RR1 (st',i') (st'',i''))
+      (LE: rcompose RR0 RR1 <2= RR)
+    :
+    sim_strict_transC r R RR (st, i) (st'', i'')
+  .
+
+  Lemma sim_strict_transC_mon
+        r1 r2
+        (LEr: r1 <4= r2)
+    :
+    sim_strict_transC r1 <4= sim_strict_transC r2
+  .
+  Proof. ii. destruct PR; econs; et. Qed.
+
+  Lemma sim_strict_transC_wrespectful:
+    wrespectful4 _sim_strict sim_strict_transC.
+  Proof.
+    econs; eauto using sim_strict_transC_mon; i.
+    destruct PR. apply GF in REL0. apply GF in REL1.
+    inv REL0; grind; depdes H3 H0; grind; unfold trigger in *; try (rewrite !bind_vis in x; depdes x);
+      inv REL1; grind; depdes H3 H0; grind; unfold trigger in *; try (rewrite !bind_vis in x; depdes x);
+      econs; i; eauto using sim_strict_transC, rclo4.
+    - replace k' with k0 in K; eauto using sim_strict_transC, rclo4.
+      extensionality v. eapply equal_f in x. rewrite !bind_ret_l in x. eauto.
+    - replace k' with k0 in K; eauto using sim_strict_transC, rclo4.
+      extensionality v. eapply equal_f in x. rewrite !bind_ret_l in x. eauto.
+    - replace k' with k0 in K; cycle 1.
+      { extensionality v. eapply equal_f in x. rewrite !bind_ret_l in x. eauto. }
+      destruct (K0 x'), (K x0). eauto using sim_strict_transC, rclo4.
+    - replace k' with k0 in K; cycle 1.
+      { extensionality v. eapply equal_f in x. rewrite !bind_ret_l in x. eauto. }
+      destruct (K x0), (K0 x1). eauto using sim_strict_transC, rclo4.
+    - replace k' with k0 in K; cycle 1; eauto using sim_strict_transC, rclo4.
+      extensionality v. eapply equal_f in x. rewrite !bind_ret_l in x. eauto.
+  Qed.
+
+  Lemma sim_strict_transC_spec:
+    sim_strict_transC <5= gupaco4 _sim_strict (cpn4 _sim_strict).
+  Proof.
+    intros. eapply wrespect4_uclo; eauto with paco.
+    apply sim_strict_transC_wrespectful.
+  Qed.
+
+  Lemma sim_strict_inv_ret R RR sti st' v'
+      (EQV: sim_strict R RR sti (st', Ret v')):
+    exists st v, sti = (st, Ret v) /\ RR (st, v) (st', v').
+  Proof.
+    punfold EQV. inv EQV; grind; depdes H0; unfold trigger in *; eauto;
+      try (rewrite !bind_vis in x; clarify).      
+  Qed.
+
+  Lemma sim_strict_inv_ret' R RR st v sti'
+      (EQV: sim_strict R RR (st, Ret v) sti'):
+    exists st' v', sti' = (st', Ret v') /\ RR (st, v) (st', v').
+  Proof.
+    punfold EQV. inv EQV; grind; depdes H0; unfold trigger in *; eauto;
+      try (rewrite !bind_vis in x; clarify).
+  Qed.
+  
+  Lemma sim_strict_inv_call R RR sti st fn varg k'
+      (EQV: sim_strict R RR sti (st, trigger (Call fn varg) >>= k')):
+    exists k,
+    sti = (st, trigger (Call fn varg) >>= k) /\
+    forall st0 vret, sim_strict R RR (st0, k vret) (st0, k' vret).
+  Proof.
+    punfold EQV. inv EQV; grind; depdes H0 H2; unfold trigger in *; eauto;
+      try (rewrite !bind_vis in x; clarify).
+    esplits; eauto. i.
+    specialize (K st0 vret). pclearbot.
+    replace k' with k'0; eauto.
+    extensionality v. depdes H0. eapply equal_f in x.
+    rewrite !bind_ret_l in x. eauto.
+  Qed.
+
+  Lemma sim_strict_inv_call' R RR st fn varg k sti' 
+      (EQV: sim_strict R RR (st, trigger (Call fn varg) >>= k) sti'):
+    exists k',
+    sti' = (st, trigger (Call fn varg) >>= k') /\
+    forall st0 vret, sim_strict R RR (st0, k vret) (st0, k' vret).
+  Proof.
+    punfold EQV. inv EQV; grind; depdes H0; unfold trigger in *; eauto;
+      try (rewrite !bind_vis in x; clarify).
+    esplits; eauto. i.
+    specialize (K st0 vret). pclearbot.
+    replace k with k0; eauto.
+    extensionality v. depdes H0. eapply equal_f in x.
+    rewrite !bind_ret_l in x. eauto.
+  Qed.
+  
+  Lemma sim_strict_inv_syscall R RR sti st' fn varg rvs k'
+      (EQV: sim_strict R RR sti (st', trigger (Syscall fn varg rvs) >>= k')):
+    exists st k,
+    sti = (st, trigger (Syscall fn varg rvs) >>= k) /\
+    forall vret, sim_strict R RR (st, k vret) (st', k' vret).
+  Proof.
+    punfold EQV. inv EQV; grind; depdes H0 H2; unfold trigger in *; eauto;
+      try (rewrite !bind_vis in x; clarify).
+    esplits; eauto. i.
+    specialize (K vret). pclearbot.
+    replace k' with k'0; eauto.
+    extensionality v. depdes H0. eapply equal_f in x.
+    rewrite !bind_ret_l in x. eauto.
+  Qed.
+
+  Lemma sim_strict_inv_syscall' R RR st fn varg rvs k sti'
+      (EQV: sim_strict R RR (st, trigger (Syscall fn varg rvs) >>= k) sti'):
+    exists st' k',
+    sti' = (st', trigger (Syscall fn varg rvs) >>= k') /\
+    forall vret, sim_strict R RR (st, k vret) (st', k' vret).
+  Proof.
+    punfold EQV. inv EQV; grind; depdes H0; unfold trigger in *; eauto;
+      try (rewrite !bind_vis in x; clarify).
+    esplits; eauto. i.
+    specialize (K vret). pclearbot.
+    replace k with k0; eauto.
+    extensionality v. depdes H0. eapply equal_f in x.
+    rewrite !bind_ret_l in x. eauto.
+  Qed.
+  
+  Lemma sim_strict_inv_tau R RR sti st' i'
+      (EQV: sim_strict R RR sti (st', tau;; i')):
+    exists st i,
+    sti = (st, tau;; i) /\
+    sim_strict R RR (st, i) (st', i').
+  Proof.
+    punfold EQV. inv EQV; grind; depdes H0; unfold trigger in *; eauto;
+      try (rewrite !bind_vis in x; clarify).
+    pclearbot. eauto.
+  Qed.
+
+  Lemma sim_strict_inv_tau' R RR st i sti' 
+      (EQV: sim_strict R RR (st, tau;; i) sti'):
+    exists st' i',
+    sti' = (st', tau;; i') /\
+    sim_strict R RR (st, i) (st', i').
+  Proof.
+    punfold EQV. inv EQV; grind; depdes H0; unfold trigger in *; eauto;
+      try (rewrite !bind_vis in x; clarify).
+    pclearbot. eauto.
+  Qed.
+  
+  Lemma sim_strict_inv_choose R RR sti st' X' k'
+      (EQV: sim_strict R RR sti (st', trigger (Choose X') >>= k')):
+    exists st X k,
+    sti = (st, trigger (Choose X) >>= k) /\
+    forall x', exists x, sim_strict R RR (st, k x) (st', k' x').
+  Proof.
+    punfold EQV. inv EQV; grind; depdes H0 H2; unfold trigger in *; eauto;
+      try (rewrite !bind_vis in x; clarify).
+    replace k' with k'0; cycle 1.
+    { depdes H0. extensionality v. eapply equal_f in x.
+      rewrite !bind_ret_l in x. eauto. }
+    esplits; eauto.
+    i. specialize (K x'). des. pclearbot. eauto.
+  Qed.
+
+  Lemma sim_strict_inv_choose' R RR st X k sti' 
+      (EQV: sim_strict R RR (st, trigger (Choose X) >>= k) sti'):
+    exists st' X' k',
+    sti' = (st', trigger (Choose X') >>= k') /\
+    forall x', exists x, sim_strict R RR (st, k x) (st', k' x').
+  Proof.
+    punfold EQV. inv EQV; grind; depdes H0; unfold trigger in *; eauto;
+      try (rewrite !bind_vis in x; clarify).
+    replace k with k0; cycle 1.
+    { depdes H0. extensionality v. eapply equal_f in x.
+      rewrite !bind_ret_l in x. eauto. }
+    esplits; eauto.
+    i. specialize (K x'). des. pclearbot. eauto.
+  Qed.
+  
+  Lemma sim_strict_inv_take R RR sti st' X' k'
+      (EQV: sim_strict R RR sti (st', trigger (Take X') >>= k')):
+    exists st X k,
+    sti = (st, trigger (Take X) >>= k) /\
+    forall x, exists x', sim_strict R RR (st, k x) (st', k' x').
+  Proof.
+    punfold EQV. inv EQV; grind; depdes H0 H2; unfold trigger in *; eauto;
+      try (rewrite !bind_vis in x; clarify).
+    replace k' with k'0; cycle 1.
+    { depdes H0. extensionality v. eapply equal_f in x.
+      rewrite !bind_ret_l in x. eauto. }
+    esplits; eauto.
+    i. specialize (K x). des. pclearbot. eauto.
+  Qed.
+
+  Lemma sim_strict_inv_take' R RR st X k sti'
+      (EQV: sim_strict R RR (st, trigger (Take X) >>= k) sti'):
+    exists st' X' k',
+    sti' = (st', trigger (Take X') >>= k') /\
+    forall x, exists x', sim_strict R RR (st, k x) (st', k' x').
+  Proof.
+    punfold EQV. inv EQV; grind; depdes H0; unfold trigger in *; eauto;
+      try (rewrite !bind_vis in x; clarify).
+    replace k with k0; cycle 1.
+    { depdes H0. extensionality v. eapply equal_f in x.
+      rewrite !bind_ret_l in x. eauto. }
+    esplits; eauto.
+    i. specialize (K x). des. pclearbot. eauto.
+  Qed.
+  
+  Lemma sim_strict_inv_update R RR sti st' X' (run': Any.t -> Any.t * X') k'
+      (EQV: sim_strict R RR sti (st', trigger (SUpdate run') >>= k')):
+    exists X (run: Any.t -> Any.t * X) st k,
+    sti = (st, trigger (SUpdate run) >>= k) /\
+    sim_strict R RR ((run st).1, k (run st).2) ((run' st').1, k' (run' st').2).
+  Proof.
+    punfold EQV. inv EQV; grind; depdes H0 H2; unfold trigger in *; eauto;
+      try (rewrite !bind_vis in x; clarify).
+    replace k' with k'0; cycle 1.
+    { depdes H0. extensionality v. eapply equal_f in x.
+      rewrite !bind_ret_l in x. eauto. }
+    depdes H1. pclearbot. esplits; eauto.
+  Qed.
+
+  Lemma sim_strict_inv_update' R RR st X (run: Any.t -> Any.t * X) k sti'
+      (EQV: sim_strict R RR (st, trigger (SUpdate run) >>= k) sti'):
+    exists X' (run': Any.t -> Any.t * X') st' k',
+    sti' = (st', trigger (SUpdate run') >>= k') /\
+    sim_strict R RR ((run st).1, k (run st).2) ((run' st').1, k' (run' st').2).
+  Proof.
+    punfold EQV. inv EQV; grind; depdes H0; unfold trigger in *; eauto;
+      try (rewrite !bind_vis in x; clarify).
+    replace k with k0; cycle 1.
+    { depdes H0. extensionality v. eapply equal_f in x.
+      rewrite !bind_ret_l in x. eauto. }
+    depdes H1. pclearbot. esplits; eauto.
+  Qed.
+
+  (** **)
+
+  Variant sim_strictC
+      (r: forall S_src S_tgt (RR: Any.t -> Any.t -> S_src -> S_tgt -> Prop), bool -> bool -> Σ -> Any.t * itree Es S_src -> Any.t * itree Es S_tgt -> Prop):
+      forall S_src S_tgt (RR: Any.t -> Any.t -> S_src -> S_tgt -> Prop), bool -> bool -> Σ -> Any.t * itree Es S_src -> Any.t * itree Es S_tgt -> Prop
+    :=
+  | sim_strictC_intro RR f_src f_tgt w sti_src sti_tgt sti_src' sti_tgt'
+      (SIM: r Any.t Any.t RR f_src f_tgt w sti_src' sti_tgt')
+      (EQVSRC: sim_strict Any.t eq sti_src sti_src')
+      (EQVTGT: sim_strict Any.t eq sti_tgt' sti_tgt)
+    : sim_strictC r Any.t Any.t RR f_src f_tgt w sti_src sti_tgt
+  .
+
+  Lemma sim_strictC_mon r1 r2
+    (LEr: r1 <8= r2)
+    :
+    sim_strictC r1 <8= sim_strictC r2.
+  Proof. ii. destruct PR. econs; et. Qed.
+
+  Lemma sim_strictC_compatible: forall wf le fl_src fl_tgt, 
+      compatible8 (@_sim_itree Σ wf le fl_src fl_tgt) sim_strictC.
+  Proof.
+    econs; i; eauto using sim_strictC_mon. depdes PR.
+    move SIM before RR. revert_until SIM.
+    induction SIM; i; subst.
+    - apply sim_strict_inv_ret in EQVSRC. apply sim_strict_inv_ret' in EQVTGT.
+      des. subst. clarify. eauto using _sim_itree.
+    - apply sim_strict_inv_call in EQVSRC. apply sim_strict_inv_call' in EQVTGT.
+      des. subst. clarify. eauto using _sim_itree.
+    - apply sim_strict_inv_syscall in EQVSRC. apply sim_strict_inv_syscall' in EQVTGT.
+      des. subst. eauto using _sim_itree.
+    - apply sim_strict_inv_call in EQVSRC. des. subst.
+      destruct sti_tgt. econs; eauto. eapply IHSIM; eauto.
+      ginit. guclo sim_strict_bindC_spec. econs.
+      + gfinal. right. eapply sim_strict_refl.
+      + i. inv REL. gfinal. right. apply EQVSRC0.
+    - apply sim_strict_inv_call' in EQVTGT. des. subst.
+      destruct sti_src. econs; eauto. eapply IHSIM; eauto.
+      ginit. guclo sim_strict_bindC_spec. econs.
+      + gfinal. right. eapply sim_strict_refl.
+      + i. inv REL. gfinal. right. apply EQVTGT0.
+    - apply sim_strict_inv_tau in EQVSRC. des. subst.
+      destruct sti_tgt. econs; eauto.
+    - apply sim_strict_inv_tau' in EQVTGT. des. subst.
+      destruct sti_src. econs; eauto.
+    - apply sim_strict_inv_choose in EQVSRC. des. subst.
+      specialize (EQVSRC0 x). des. destruct sti_tgt. econs; eauto.
+    - apply sim_strict_inv_choose' in EQVTGT. des. subst.
+      destruct sti_src. econs; eauto. i. specialize (EQVTGT0 x). des; eauto.
+    - apply sim_strict_inv_take in EQVSRC. des. subst.
+      destruct sti_tgt. econs. i. specialize (EQVSRC0 x). des. eauto.
+    - apply sim_strict_inv_take' in EQVTGT. des. subst.
+      specialize (EQVTGT0 x). des. destruct sti_src. econs; eauto.
+    - apply sim_strict_inv_update in EQVSRC. des. subst.
+      destruct sti_tgt. econs; eauto.
+    - apply sim_strict_inv_update' in EQVTGT. des. subst.
+      destruct sti_src. econs; eauto.
+    - destruct sti_src, sti_tgt. econs; eauto. econs; eauto.
+  Qed.
+
+  Lemma sim_strictC_spec: forall wf le fl_src fl_tgt,
+      sim_strictC <9= gupaco8 (@_sim_itree Σ wf le fl_src fl_tgt) (cpn8 (@_sim_itree Σ wf le fl_src fl_tgt)).
+  Proof.
+    intros. gclo. econs; eauto using sim_strictC_compatible.
+    eapply sim_strictC_mon, PR; eauto with paco.
+  Qed.
+
+  (** **)
+  
+  Lemma case_itrH R (itrH: itree hAGEs R) :
+    (exists v, itrH = Ret v) \/
+    (exists itrH', itrH = tau;; itrH') \/
+    (exists P itrH', itrH = (trigger (Assume P);;; itrH')) \/
+    (exists P itrH', itrH = (trigger (Guarantee P);;; itrH')) \/
+    (exists R (c: callE R) ktrH', itrH = (trigger c >>= ktrH')) \/
+    (exists R (s: sE R) ktrH', itrH = (trigger s >>= ktrH')) \/
+    (exists R (e: eventE R) ktrH', itrH = (trigger e >>= ktrH')).
+  Proof.
+    ides itrH; eauto.
+    right; right.
+    destruct e; [destruct h|destruct e; [|destruct s]].
+    - left. exists P, (k()). unfold trigger. rewrite bind_vis.
+      repeat f_equal. extensionality x. destruct x. rewrite bind_ret_l. eauto.
+    - right; left. exists P, (k()). unfold trigger. rewrite bind_vis.
+      repeat f_equal. extensionality x. destruct x. rewrite bind_ret_l. eauto.
+    - right; right; left. exists X, c, k. unfold trigger. rewrite bind_vis.
+      repeat f_equal. extensionality x. rewrite bind_ret_l. eauto.
+    - right; right; right; left. exists X, s, k. unfold trigger. rewrite bind_vis.
+      repeat f_equal. extensionality x. rewrite bind_ret_l. eauto.
+    - right; right; right; right. exists X, e, k. unfold trigger. rewrite bind_vis.
+      repeat f_equal. extensionality x. rewrite bind_ret_l. eauto.
+  Qed.
+
+  Definition hp_reconf_eq cr : relation (Any.t * Σ) :=
+    fun '(str,fr) '(str',fr') =>
+      <<RELr: Own fr ⊢ #=> Own (fr' ⋅ cr)>> /\      
+      <<STR: str' = str>>.
+  
+  Definition hp_reconf_equiv cr : relation (Any.t * Σ) :=
+    fun '(str,fr) '(str',fr') =>
+      hp_reconf_eq cr (str,fr) (str',fr')
+      \/
+      (exists st (mr mr': Σ),
+       <<RELr: Own (fr ⋅ mr) ⊢ #=> Own (fr' ⋅ mr' ⋅ cr)>> /\
+       <<STR: str = Any.pair st mr↑>> /\
+       <<STR': str' = Any.pair st mr'↑>>).
+
+  Definition hp_reconf_rel R (eqv: Σ -> _) cr : relation (Any.t * (Σ * R)) :=
+    fun '(str,(fr,x)) '(str',(fr',x')) =>
+      eqv cr (str,fr) (str',fr') /\ x = x'.
+
+  Lemma hp_reconf_equiv_strong
+    cr str str' (fr fr': Σ)
+    (EQV: hp_reconf_equiv cr (str,fr) (str',fr'))
+    :
+    (hp_reconf_eq cr (str,fr) (str',fr') /\
+     <<FAIL: ~ exists st (mr:Σ), str = Any.pair st mr↑>>)
+    \/
+    (exists st (mr mr': Σ),
+     <<RELr: Own (fr ⋅ mr) ⊢ #=> Own (fr' ⋅ mr' ⋅ cr)>> /\
+     <<STR: str = Any.pair st mr↑>> /\
+     <<STR': str' = Any.pair st mr'↑>>).
+  Proof.
+    ss. des; subst; [|right]; esplits; eauto.
+    destruct (classic (exists stx (mrx:Σ), str = Any.pair stx mrx↑)); eauto.
+    des. subst. right. esplits; eauto.
+    eapply own_ctx with (ctx := mrx) in RELr. revert RELr. r_solve. i.
+    rewrite-> URA.add_comm, (URA.add_comm fr' mrx). eauto.
+  Qed.
+  
+  Lemma hp_reconf_fail
+    r R RR str i i'
+    (FAIL: ~ exists st (mr:Σ), str = Any.pair st mr↑)
+    :
+    paco4 _sim_strict r R RR
+      (str, p <- unwrapU (Any.split str);;
+            mr <- (let '(st,_mr) := p in unwrapU (@Any.downcast Σ _mr));; i mr)
+      (str, p <- unwrapU (Any.split str);;
+            mr <- (let '(st,_mr) := p in unwrapU (@Any.downcast Σ _mr));; i' mr).
+  Proof.
+    destruct (Any.split str) eqn:STR; cycle 1.
+    { ss. unfold triggerUB. grind. pstep. econs. i. inv x. }
+    grind. destruct (Any.downcast t0) eqn:T0; cycle 1.
+    { ss. unfold triggerUB. grind. pstep. econs. i. inv x. }
+    apply Any.split_pair in STR. apply Any.downcast_upcast in T0.
+    exfalso. eapply FAIL. des; subst. eauto.
+  Qed.
+
+  Lemma handle_Guarantee_reconf
+    P str str' (fr fr' cr: Σ)
+    (RELr: hp_reconf_equiv cr (str,fr) (str',fr'))
+    :
+    sim_strict _ (hp_reconf_rel _ hp_reconf_equiv cr)
+      (str, handle_Guarantee P fr)
+      (str', handle_Guarantee P fr').
+  Proof.
+    ginit. unfold handle_Guarantee, guarantee, mget, mput.
+    grind; gstep; econs; i. destruct x' as [[c0 c1] c2]. exists (c0, c1, c2⋅cr).
+    grind; gstep; econs; i.
+    grind; apply hp_reconf_equiv_strong in RELr; repeat (rr in RELr; des; subst).
+    { gfinal. right. apply hp_reconf_fail. eauto. }
+    rewrite !Any.pair_split. grind. rewrite !Any.upcast_downcast.
+    grind; gstep; econs; i. eexists.
+    { r_solve. iIntros "H". iPoseProof (RELr0 with "H") as "H". iMod "H".
+      iDestruct "H" as "[X Y]". iSplitL "X"; eauto.
+      iPoseProof (x' with "X") as "X". eauto. }
+    grind; gstep; econs; i. eexists. { eauto. }
+    grind; gstep; econs; i. grind. rewrite !Any.pair_split.
+    repeat (grind; gstep; econs; i).
+    split; eauto. right. esplits; eauto.
+    r_solve. eauto.
+  Qed.
+
+  Lemma handle_Guarantee_reconf_true
+    str str' (fr fr' cr: Σ)
+    (RELr: hp_reconf_equiv cr (str,fr) (str',fr'))
+    :
+    sim_strict _ (hp_reconf_rel _ hp_reconf_eq cr)
+      (str, handle_Guarantee True fr)
+      (str', handle_Guarantee True fr').
+  Proof.
+    ginit. unfold handle_Guarantee, guarantee, mget, mput.
+    grind; gstep; econs; i. destruct x' as [[c0 c1] c2]. exists (c0, c1⋅cr, c2).
+    grind; gstep; econs; i.
+    grind; apply hp_reconf_equiv_strong in RELr; repeat (rr in RELr; des; subst).
+    { gfinal. right. apply hp_reconf_fail. eauto. }
+    rewrite !Any.pair_split. grind. rewrite !Any.upcast_downcast.
+    grind; gstep; econs; i. eexists.
+    { r_solve. iIntros "H". iPoseProof (RELr0 with "H") as "H". iMod "H".
+      iDestruct "H" as "[X Y]".
+      rewrite -URA.add_assoc (URA.add_comm cr c2) URA.add_assoc.
+      iSplitL "X"; eauto. iPoseProof (x' with "X") as "X". eauto. }
+    grind; gstep; econs; i. eexists. { eauto. }
+    grind; gstep; econs; i. grind. rewrite !Any.pair_split.
+    repeat (grind; gstep; econs; i).
+    split; eauto. split; eauto.
+  Qed.
+  
+  Lemma interp_hp_reconf
+    R itrH str str' (fr fr' cr: Σ)
+    (RELr: hp_reconf_equiv cr (str,fr) (str',fr'))
+    :
+    sim_strict _ (hp_reconf_rel R hp_reconf_equiv cr)
+      (str, interp_hp itrH fr)
+      (str', interp_hp itrH fr').
+  Proof.
+    revert_until I. ginit. gcofix CIH; i.
+    assert (CASE := case_itrH _ itrH). des; subst.
+    - rewrite !interp_hp_ret.
+      gstep. econs. rr. esplits; eauto.
+    - rewrite-> !interp_hp_tau.
+      grind; gstep; econs; i. eauto 10 with paco.
+    - rewrite-> !interp_hp_bind, !interp_hp_Assume.
+      unfold handle_Assume, assume, mget, mput.
+      grind; gstep; econs; i. exists x.
+      grind; gstep; econs; i.
+      grind; apply hp_reconf_equiv_strong in RELr; repeat (rr in RELr; des; subst).
+      { gfinal. right. apply hp_reconf_fail. eauto. }
+      rewrite !Any.pair_split. grind. rewrite !Any.upcast_downcast.
+      grind; gstep; econs; i. eexists.
+      { eapply own_ctx with (ctx := x) in RELr0. rewrite !URA.add_assoc in RELr0.
+        eapply own_wf in RELr0; eauto. eapply URA.wf_mon; eauto. }
+      grind; gstep; econs; i. eexists. { eauto. }
+      grind; gstep; econs; i.
+      gfinal. left. eapply CIH. right. esplits; eauto.
+      { eapply own_ctx with (ctx := x) in RELr0.
+        rewrite !URA.add_assoc in RELr0. eauto using own_wf. }
+    - rewrite-> !interp_hp_bind, !interp_hp_Guarantee. grind.
+      guclo sim_strict_bindC_spec. econs.
+      { gfinal. right. eapply paco4_mon_bot; eauto.
+        eapply handle_Guarantee_reconf. eauto. }
+      i. grind; gstep; econs; i.
+      gfinal. left. eapply CIH. destruct v0, v0'. rr in REL. des; subst. ss.
+    - rewrite-> !interp_hp_bind, !interp_hp_call. grind.
+      guclo sim_strict_bindC_spec. econs.
+      { gfinal. right. eapply paco4_mon_bot; eauto.
+        eapply handle_Guarantee_reconf_true. eauto. }
+      i. destruct v0, v0', c. repeat (rr in REL; des; subst).
+      repeat (grind; gstep; econs; i).
+      gfinal. left. eapply CIH. left. s. eauto.
+    - rewrite-> !interp_hp_bind, !interp_hp_triggerp.
+      destruct s. unfold handle_sE_tgt, pupdate.
+      repeat (grind; gstep; econs; i).
+      grind; apply hp_reconf_equiv_strong in RELr; repeat (rr in RELr; des; subst); cycle 1.
+      { rewrite !Any.pair_split. grind.
+        gfinal. left. eapply CIH. right. esplits; eauto. }
+      gfinal. left. eapply CIH.
+      destruct (Any.split str) as [[]|] eqn: STR.
+      { left. s. esplits; eauto. }
+      left. s. esplits; eauto.
+    - rewrite-> !interp_hp_bind, !interp_hp_triggere.
+      destruct e.
+      + grind; gstep; econs; i. eexists.
+        repeat (grind; gstep; econs; i). eauto 10 with paco.
+      + grind; gstep; econs; i. eexists.
+        repeat (grind; gstep; econs; i). eauto 10 with paco.
+      + repeat (grind; gstep; econs; i). eauto 10 with paco.
+  Qed.
+
+  Lemma hp_fun_tail_reconf
+    str str' (fr fr' cr: Σ) x
+    (RELr: hp_reconf_equiv cr (str,fr) (str',fr'))
+    :
+    sim_strict _ eq
+      (str, hp_fun_tail (fr,x))
+      (str', hp_fun_tail (fr',x)).
+  Proof.
+    ginit. unfold hp_fun_tail. guclo sim_strict_bindC_spec. econs.
+    { gfinal. right. eapply handle_Guarantee_reconf_true. eauto. }
+    i. destruct v0, v0'. repeat (rr in REL; des; subst).
+    eauto with paco.
+  Qed.
+
+  Lemma interp_hp_body_reconf
+    itrH str str' (fr fr' cr: Σ)
+    (RELr: hp_reconf_equiv cr (str,fr) (str',fr'))
+    :
+    sim_strict _ eq
+      (str, interp_hp_body itrH fr)
+      (str', interp_hp_body itrH fr').
+  Proof.
+    ginit. unfold interp_hp_body.
+    guclo sim_strict_bindC_spec. econs.
+    { gfinal. right. eapply interp_hp_reconf. eauto. }
+    i. destruct v0, v0'. repeat (rr in REL; des; subst); cycle 1.
+    - gfinal. right. eapply hp_fun_tail_reconf. right. esplits; eauto.
+    - gfinal. right. eapply hp_fun_tail_reconf. left. esplits; eauto.
+      rr. esplits; eauto.
+  Qed.
+
+  Lemma interp_strict_inline_src
+    itrH ktrH st (fr mr: Σ)
+    :
+    sim_strict Any.t eq
+      (Any.pair st (fr ⋅ mr)↑, x <- interp_hp_body itrH ε;; '(rr,rv) <- (tau;; Ret (ε,x));; interp_hp_body (ktrH rv) rr)
+      (Any.pair st mr↑, interp_hp_body (x <- itrH;; trigger (Guarantee (True%I)) ;;; ktrH x) fr).
+  Proof.
+    ginit. guclo sim_strict_transC_spec. econs; cycle 1.
+    { gfinal. right. eapply interp_hp_body_reconf with (fr := (ε:Σ)) (cr:=(ε:Σ)).
+      right. esplits; eauto. instantiate (1:= fr ⋅ mr). r_solve. eauto. }
+    { i. destruct PR. subst. eauto. }
+    unfold interp_hp_body. rewrite !interp_hp_bind.
+    grind. guclo sim_strict_bindC_spec. econs.
+    { gfinal. right. apply sim_strict_refl. }
+    i. depdes REL. rewrite-> interp_hp_bind, interp_hp_Guarantee.
+    destruct v0' as [fr' st']. unfold hp_fun_tail at 1. grind.
+    unfold handle_Guarantee, mget, mput, guarantee, sGet, sPut.
+    grind; gstep; econs; i. destruct x' as [[c0 c1] c2]. exists (c0, ε, c1 ⋅ c2).
+    grind; gstep; econs; i.
+    ss. destruct (Any.split st0') eqn: ST0'; ss; cycle 1.
+    { unfold triggerUB. grind; gstep; econs. i. inv x. }
+    grind. destruct (Any.downcast t0) eqn: T0; ss; cycle 1.
+    { unfold triggerUB. grind; gstep; econs. i. inv x. }
+    apply Any.split_pair in ST0'. rr in ST0'. subst.
+    apply Any.downcast_upcast in T0. rr in T0. subst.
+    grind; gstep; econs; i. eexists. { r_solve. eauto. }
+    grind; gstep; econs; i. eexists. { eauto. }
+    repeat (grind; gstep; econs; i).
+    grind. rewrite !Any.pair_split.
+    repeat (grind; gstep; econs; i).
+    gfinal. right. eapply interp_hp_body_reconf with (cr:=(ε:Σ)).
+    right. esplits; eauto. r_solve. eauto.
+  Qed.
+
+  Lemma interp_strict_inline_tgt
+    itrH ktrH st (fr mr fr' mr': Σ)
+    (RELr: Own (fr ⋅ mr) ⊢ #=> Own (fr' ⋅ mr'))
+    :
+    sim_strict Any.t eq
+      (Any.pair st mr↑, interp_hp_body (x <- itrH;; trigger (Guarantee (True%I)) ;;; ktrH x) fr)
+      (Any.pair st mr'↑, x <- interp_hp_body itrH ε;; '(rr,rv) <- (tau;; Ret (fr',x));; interp_hp_body (ktrH rv) rr).
+  Proof.
+    ginit. unfold interp_hp_body. rewrite-> !interp_hp_bind. grind.
+    guclo sim_strict_bindC_spec. econs.
+    { gfinal. right. eapply interp_hp_reconf with (cr:=fr').
+      right. esplits; eauto. r_solve.
+      rewrite (URA.add_comm mr' fr'). eauto. }
+    i. rewrite-> !interp_hp_bind, interp_hp_Guarantee. unfold hp_fun_tail. grind.
+    guclo sim_strict_bindC_spec. econs.
+    { gfinal. right. eapply handle_Guarantee_reconf_true.
+      destruct v0. ss. des; subst; eauto.
+      right. esplits; eauto. }
+    i. grind; gstep; econs; i.
+    destruct v0. rr in REL; des; subst. simpl. destruct v1, v0'.
+    guclo sim_strict_bindC_spec. econs.
+    { gfinal. right.  eapply interp_hp_reconf with (cr:=c2).
+      s in REL0; des; subst. left. s. esplits; eauto.
+      rewrite URA.add_comm. eauto. }
+    i. grind. guclo sim_strict_bindC_spec. econs.
+    { gfinal. right. eapply handle_Guarantee_reconf_true.
+      r in REL1. des; subst. eauto. }
+    i. gstep; econs. rr in REL1. des; subst.
+    destruct v0, v0'. s in REL2; des; subst. eauto. 
+  Qed.
+
+
+  (*** ****)
+  
+  
+  Variant interp_inv: Σ -> Any.t * Any.t -> Prop :=
+    | interp_inv_intro
+        (ctx mr_src mr_tgt: Σ) st_src st_tgt mr
+        (WF: URA.wf (ctx ⋅ mr_src))
+        (MRS: Own mr_src ⊢ #=> Own (mr ⋅ mr_tgt))
+        (MR: Own mr ⊢ #=> I st_src st_tgt)
+      :
+      interp_inv ctx (Any.pair st_src mr_src↑, Any.pair st_tgt mr_tgt↑)
+  .
+  
+  Lemma hpsim_adequacy:
+    forall
+      (fl_src0 fl_tgt0: alist string (Any.t -> itree Es Any.t)) 
+      (FLS: fl_src0 = List.map (fun '(s, f) => (s, interp_hp_fun f)) fl_src)
+      (FLT: fl_tgt0 = List.map (fun '(s, f) => (s, interp_hp_fun f)) fl_tgt)
+      f_src f_tgt st_src st_tgt itr_src itr_tgt
+      (ctx mr_src mr_tgt fr_src fr_tgt fmr: Σ)
+      (SIM: hpsim f_src f_tgt (st_src, itr_src) (st_tgt, itr_tgt) fmr)
+      (WF: URA.wf (ctx ⋅ fr_src ⋅ mr_src))
+      (FMR: Own (fr_src ⋅ mr_src) ⊢ #=> Own (fmr ⋅ fr_tgt ⋅ mr_tgt)),
+    @sim_itree Σ interp_inv (fun _ _ => True) fl_src0 fl_tgt0 f_src f_tgt ctx
+      (Any.pair st_src mr_src↑, interp_hp_body itr_src fr_src)
+      (Any.pair st_tgt mr_tgt↑, interp_hp_body itr_tgt fr_tgt).
+  Proof.
+    i. revert_until I. ginit. gcofix CIH. i.
+    remember (st_src, itr_src). remember (st_tgt, itr_tgt).
+    move SIM before FLT. revert_until SIM.
+    punfold SIM. induction SIM; i; clarify.
     - admit.
     - admit.
     - admit.
-    - admit.
-    - admit.
-    - admit.
+    - exploit IHSIM; eauto. i.
+      rewrite-> interp_hp_body_bind, interp_hp_call.
+      unfold handle_Guarantee, mget, mput, guarantee. 
+      steps. force_l. instantiate (1:= (ε, ε, fr_src ⋅ mr_src)).
+      steps. force_l. { r_solve; et. }
+      steps. force_l; et. steps.
+      {	instantiate (1:= interp_hp_fun f).
+	rewrite alist_find_map. rewrite FUN. et. }
+      guclo sim_strictC_spec. econs; eauto.
+      + apply interp_strict_inline_src.
+      + apply sim_strict_refl.
+    - exploit IHSIM; eauto. i.
+      rewrite-> interp_hp_body_bind, interp_hp_call.
+      unfold handle_Guarantee, mget, mput, guarantee.
+      steps.
+      {	instantiate (1:= interp_hp_fun f).
+	rewrite alist_find_map. rewrite FUN. et. }
+      guclo sim_strictC_spec. econs; eauto.
+      + apply sim_strict_refl.      
+      + apply interp_strict_inline_tgt.
+        { iIntros "H". iPoseProof (x with "H") as "H". iMod "H".
+          iDestruct "H" as "[[X Y] Z]". iModIntro. iSplitL "Y"; eauto. }
     - 
+
+
+
+
+
+
+
+
+      
+
+      
+
       
       
-
-      depdes Heqsitr_src. depdes LE_src.
-      + 
-
-      rewrite <-x0 in x1.
+      unfold interp_hp_fun.
       
-		- ides itr0; depdes H0; revert x; grind. 
-			2: { rewrite bind_vis in x. clarify. }
-			unfold handle_Guarantee, guarantee, mget, mput. grind. 
-			eapply sim_itree_choose_src. instantiate (1:= (ε, ε, mr ⋅ c)). grind. 
-			eapply sim_itree_supdate_src. grind.
-			rewrite Any.pair_split. grind.
-			rewrite Any.upcast_downcast. grind.
-			eapply sim_itree_choose_src. { r_solve. iIntros "[H H0]". iSplitL "H0"; et. }
-			eapply sim_itree_choose_src; et.
-			eapply sim_itree_supdate_src. grind.
-			rewrite Any.pair_split. grind.
-			eapply sim_itree_supdate_src. grind.
-			eapply sim_itree_tau_src. ss.
-			admit.
-			
-		- ides itr0; cycle 1.
-			{ (* tau *) revert H1; grind. rewrite bind_trigger in H1. clarify. }
-			{ (* vis *)
-				(* grind. rewrite bind_vis. *)
-				rewrite bind_vis in H1.
-				rewrite bind_trigger in H1. admit.
-			}
-			admit.
-		- admit.
-		- admit.
-		- eapply sim_itree_inline_tgt; et.
-		- ides itr0; revert H0; grind; cycle 2.
-			{ rewrite bind_vis in H0. clarify. }
-			{ 
-				unfold handle_Guarantee, mget, mput, guarantee. grind.
-				eapply sim_itree_choose_src. instantiate (1:= (ε, ε, mr ⋅ c)). grind.
-				eapply sim_itree_supdate_src. grind.
-				rewrite Any.pair_split. grind.
-				rewrite Any.upcast_downcast. grind.
-				eapply sim_itree_choose_src. { r_solve. iIntros "[H H0]". iSplitL "H0"; et. }
-				eapply sim_itree_choose_src; et.
-				eapply sim_itree_supdate_src. grind.
-				rewrite Any.pair_split. grind.
-				eapply sim_itree_supdate_src. grind.
-				eapply sim_itree_tau_src. ss.
-				admit.
-			}
-			eapply sim_itree_tau_src.
-			
-		- eapply sim_itree_tau_tgt; et.
-		- admit.
-		- eapply sim_itree_choose_tgt; et.
-			
-
-	Qed.
-
-
-	End INLINEC.
-
-
-	Lemma interp_hp_fun_bind
-      (R S: Type)
-      (s : itree hAGEs R) (k : R -> itree hAGEs S)
-      fmr
-  :
-    (interp_hp_fun (s >>= k) fmr)
-    =
-    st <- interp_hp s fmr;; interp_hp_fun (k st.2) st.1.
-Proof.
-	unfold interp_hp_fun. rewrite interp_hp_bind. grind.
-Qed.
-
-
-Variant mk_inv  
-(I: Any.t -> Any.t -> iProp)
-: Σ -> Any.t * Any.t -> Prop :=
-| mk_inv_intro
-(ctx mr_src mr_tgt: Σ) st_src st_tgt
-(INV: exists mr,
-	<<WF: URA.wf (ctx ⋅ mr_src)>> /\
-	<<MRS: Own mr_src ⊢ #=> Own (mr ⋅ mr_tgt)>> /\
-	<<MR: Own mr ⊢ #=> (I st_src st_tgt)>>)
-:
-mk_inv I ctx (Any.pair st_src mr_src↑, Any.pair st_tgt mr_tgt↑)
-.
-
-
-	Lemma hpsim_adequacy:
-	forall
-	(fl_src0 fl_tgt0: alist string (Any.t -> itree Es Any.t)) 
-	(FLS: fl_src0 = List.map (fun '(s, f) => (s, interp_hp_fun f)) fl_src)
-	(FLT: fl_tgt0 = List.map (fun '(s, f) => (s, interp_hp_fun f)) fl_tgt)
-	f_src f_tgt st_src st_tgt itr_src itr_tgt
-	(ctx mr_src mr_tgt fr_src fr_tgt fmr: Σ)
-	(SIM: hpsim f_src f_tgt (st_src, itr_src) (st_tgt, itr_tgt) fmr)
-	(WF: URA.wf (ctx ⋅ fr_src ⋅ mr_src))
-	(FMR: Own (fr_src ⋅ mr_src) ⊢ #=> Own (fmr ⋅ fr_tgt ⋅ mr_tgt)),
-
-
-		@sim_itree Σ (mk_inv I) (fun _ _ => True) fl_src0 fl_tgt0 f_src f_tgt ctx
-		(Any.pair st_src mr_src↑, (interp_hp_fun itr_src fr_src) >>= (fun r => Ret (snd r)))
-		(Any.pair st_tgt mr_tgt↑, (interp_hp_fun itr_tgt fr_tgt) >>= (fun r => Ret (snd r))).
-Proof.
-	i. 
-	(* remember (Any.pair st_src mr_src↑). remember (Any.pair st_tgt mr_tgt↑). *)
-	revert_until I.
-	ginit. gcofix CIH. i.
-	remember (st_src, itr_src). remember (st_tgt, itr_tgt).
-	move SIM before FLT. revert_until SIM.	
-
-	induction SIM using hpsim_ind; i; clarify. 
-	4:{
-		rewrite interp_hp_fun_bind.
-		(* unfold interp_hp_fun. *)
-
-		steps. unfold handle_Guarantee at 1. unfold mget, mput, guarantee. 
-		steps. force_l. instantiate (1:= (ε, ε, fr_src ⋅ mr_src)).
-		steps. force_l. 
-		{ r_solve; et. }
-		steps. force_l; et. 
-		steps.
-		{
-			instantiate (1:= interp_hp_fun f).
-			rewrite alist_find_map. rewrite FUN. et.
-		}
-		rewrite <- bind_bind. 
+      
+      rewrite !bind_bind. 
 		unfold interp_hp_fun.
 		gclo. eapply compatible'8_companion; eauto with paco.
 		{ eapply compat8_compatible'. apply inlineSrcC_compatible. }	
